Simplify frac : use a pair of a rational and a carrier

algebra/frac.v
@@ -5,207 +5,37 @@ Local Arguments op _ _ !_ !_ /.
 Local Arguments validN _ _ _ !_ /.
 Local Arguments valid _ _  !_ /.
 
-Inductive frac A := Frac { frac_perm : Qp ; frac_car : A  }.
-Add Printing Constructor frac.
-Arguments Frac {_} _ _.
-Arguments frac_perm {_} _.
-Arguments frac_car {_} _.
-Instance: Params (@Frac) 2.
+Notation frac := Qp.
 
-Section cofe.
-Context {A : cofeT}.
-Implicit Types a b : A.
-Implicit Types x y : frac A.
+Section frac.
 
-(* Cofe *)
-Instance frac_equiv : Equiv (frac A) := λ x y,
-  frac_perm x = frac_perm y ∧ frac_car x ≡ frac_car y.
-Instance frac_dist : Dist (frac A) := λ n x y,
-  frac_perm x = frac_perm y ∧ frac_car x ≡{n}≡ frac_car y.
+Canonical Structure fracC := leibnizC frac.
 
-Global Instance Frac_ne q n : Proper (dist n ==> dist n) (@Frac A q).
-Proof. by constructor. Qed.
-Global Instance Frac_proper q : Proper ((≡) ==> (≡)) (@Frac A q).
-Proof. by constructor. Qed.
-Global Instance Frac_inj : Inj2 (=) (≡) (≡) (@Frac A).
-Proof. by destruct 1. Qed.
-Global Instance Frac_dist_inj n : Inj2 (=) (dist n) (dist n) (@Frac A).
-Proof. by destruct 1. Qed.
+Instance frac_valid : Valid frac := λ x, (x ≤ 1)%Qc.
+Instance frac_pcore : PCore frac := λ _, None.
+Instance frac_op : Op frac := λ x y, (x + y)%Qp.
 
-Global Instance frac_perm_ne n : Proper (dist n ==> (=)) (@frac_perm A).
-Proof. by destruct 1. Qed.
-Global Instance frac_car_ne n : Proper (dist n ==> dist n) (@frac_car A).
-Proof. by destruct 1. Qed.
-Global Instance frac_perm_proper : Proper ((≡) ==> (=)) (@frac_perm A).
-Proof. by destruct 1. Qed.
-Global Instance frac_car_proper : Proper ((≡) ==> (≡)) (@frac_car A).
-Proof. by destruct 1. Qed.
-
-Program Definition frac_chain (c : chain (frac A)) : chain A :=
-  {| chain_car n := match c n return _ with Frac _ b => b end |}.
-Next Obligation.
-  intros c n i ?; simpl. destruct (c 0) eqn:?; simplify_eq/=.
-  by feed inversion (chain_cauchy c n i).
-Qed.
-Instance frac_compl : Compl (frac A) := λ c,
-  Frac (frac_perm (c 0)) (compl (frac_chain c)).
-Definition frac_cofe_mixin : CofeMixin (frac A).
+Definition frac_ra_mixin : RAMixin frac.
 Proof.
-  split.
-  - intros mx my; split.
-    + by destruct 1; subst; constructor; try apply equiv_dist.
-    + intros Hxy; feed inversion (Hxy 0); subst; constructor; try done.
-      apply equiv_dist=> n; by feed inversion (Hxy n).
-  - intros n; split.
-    + by intros [q a]; constructor.
-    + by destruct 1; constructor.
-    + destruct 1; inversion_clear 1; constructor; etrans; eauto.
-  - by inversion_clear 1; constructor; done || apply dist_S.
-  - intros n c; constructor; simpl.
-    + destruct (chain_cauchy c 0 n); auto with lia.
-    + apply (conv_compl n (frac_chain c)).
+  split; try apply _; try done.
+  unfold valid, op, frac_op, frac_valid. intros. trans (x+y)%Qp. 2:done.
+  rewrite -{1}(Qcplus_0_r x) -Qcplus_le_mono_l; auto using Qclt_le_weak.
 Qed.
-Canonical Structure fracC : cofeT := CofeT (frac A) frac_cofe_mixin.
-Global Instance frac_discrete : Discrete A → Discrete fracC.
-Proof. by inversion_clear 2; constructor; done || apply (timeless _). Qed.
-Global Instance frac_leibniz : LeibnizEquiv A → LeibnizEquiv (frac A).
-Proof. intros ? [??] [??] [??]; f_equal; done || by apply leibniz_equiv. Qed.
+Canonical Structure fracR := discreteR frac frac_ra_mixin.
 
-Global Instance Frac_timeless q (a : A) : Timeless a → Timeless (Frac q a).
-Proof. by inversion_clear 2; constructor; done || apply (timeless _). Qed.
-End cofe.
-
-Arguments fracC : clear implicits.
-
-(* Functor on COFEs *)
-Definition frac_map {A B} (f : A → B) (x : frac A) : frac B :=
-  match x with Frac q a => Frac q (f a) end.
-Instance: Params (@frac_map) 2.
-
-Lemma frac_map_id {A} (x : frac A) : frac_map id x = x.
-Proof. by destruct x. Qed.
-Lemma frac_map_compose {A B C} (f : A → B) (g : B → C) (x : frac A) :
-  frac_map (g ∘ f) x = frac_map g (frac_map f x).
-Proof. by destruct x. Qed.
-Lemma frac_map_ext {A B : cofeT} (f g : A → B) x :
-  (∀ x, f x ≡ g x) → frac_map f x ≡ frac_map g x.
-Proof. destruct x; constructor; simpl; auto. Qed.
-Instance frac_map_cmra_ne {A B : cofeT} n :
-  Proper ((dist n ==> dist n) ==> dist n ==> dist n) (@frac_map A B).
-Proof. intros f f' Hf [??] [??] [??]; constructor; by try apply Hf. Qed.
-Definition fracC_map {A B} (f : A -n> B) : fracC A -n> fracC B :=
-  CofeMor (frac_map f).
-Instance fracC_map_ne A B n : Proper (dist n ==> dist n) (@fracC_map A B).
-Proof. intros f f' Hf []; constructor; by try apply Hf. Qed.
-
-Section cmra.
-Context {A : cmraT}.
-Implicit Types a b : A.
-Implicit Types x y : frac A.
-
-Instance frac_valid : Valid (frac A) := λ x,
-  (frac_perm x ≤ 1)%Qc ∧ ✓ frac_car x.
-Global Arguments frac_valid !_/.
-Instance frac_validN : ValidN (frac A) := λ n x,
-  (frac_perm x ≤ 1)%Qc ∧ ✓{n} frac_car x.
-Global Arguments frac_validN _ !_/.
-Instance frac_pcore : PCore (frac A) := λ _, None.
-Instance frac_op : Op (frac A) := λ x y,
-  Frac (frac_perm x + frac_perm y) (frac_car x ⋅ frac_car y).
-Global Arguments frac_op !_ !_ /.
-
-Lemma Frac_op q1 q2 a b : Frac q1 a ⋅ Frac q2 b = Frac (q1 + q2) (a ⋅ b).
-Proof. done. Qed.
-
-Definition frac_cmra_mixin : CMRAMixin (frac A).
-Proof.
-  split; try discriminate.
-  - intros n [??] [??] [??] [??]; constructor; by cofe_subst. 
-  - intros ? [??] [??] [??] [??]; split; by cofe_subst.
-  - intros [??]; rewrite /= ?cmra_valid_validN; naive_solver eauto using O.
-  - intros n [q a]; destruct 1; split; auto using cmra_validN_S.
-  - intros [q1 a1] [q2 a2] [q3 a3]; constructor; by rewrite /= ?assoc.
-  - intros [q1 a1] [q2 a2]; constructor; by rewrite /= 1?comm ?[(q1+_)%Qp]comm.
-  - intros n [q1 a1] [q2 a2]; destruct 1; split; eauto using cmra_validN_op_l.
-    trans (q1 + q2)%Qp; simpl; last done.
-    rewrite -{1}(Qcplus_0_r q1) -Qcplus_le_mono_l; auto using Qclt_le_weak.
-  - intros n [q a] y1 y2 Hx Hx'.
-    destruct Hx, y1 as [q1 b1], y2 as [q2 b2].
-    apply (inj2 Frac) in Hx'; destruct Hx' as [-> ?].
-    destruct (cmra_extend n a b1 b2) as ([z1 z2]&?&?&?); auto.
-    exists (Frac q1 z1,Frac q2 z2); by repeat constructor.
-Qed.
-Canonical Structure fracR := CMRAT (frac A) frac_cofe_mixin frac_cmra_mixin.
-
-Global Instance frac_cmra_discrete : CMRADiscrete A → CMRADiscrete fracR.
-Proof.
-  split; first apply _.
-  intros [q a]; destruct 1; split; auto using cmra_discrete_valid.
-Qed.
+End frac.
 
 (** Internalized properties *)
-Lemma frac_equivI {M} (x y : frac A) :
-  x ≡ y ⊣⊢ (frac_perm x = frac_perm y ∧ frac_car x ≡ frac_car y : uPred M).
+Lemma frac_equivI {M} (x y : frac) :
+  x ≡ y ⊣⊢ (x = y : uPred M).
 Proof. by uPred.unseal. Qed.
-Lemma frac_validI {M} (x : frac A) :
-  ✓ x ⊣⊢ (■ (frac_perm x ≤ 1)%Qc ∧ ✓ frac_car x : uPred M).
+Lemma frac_validI {M} (x : frac) :
+  ✓ x ⊣⊢ (■ (x ≤ 1)%Qc : uPred M).
 Proof. by uPred.unseal. Qed.
 
 (** Exclusive *)
-Global Instance frac_full_exclusive a : Exclusive (Frac 1 a).
+Global Instance frac_full_exclusive : Exclusive 1%Qp.
 Proof.
-  move => [[??]?][/Qcle_not_lt[]]; simpl in *.
+  move => ? /Qcle_not_lt[]; simpl in *.
   by rewrite -{1}(Qcplus_0_r 1) -Qcplus_lt_mono_l.
-Qed.
-
-(** ** Local updates *)
-Global Instance frac_local_update `{!LocalUpdate Lv L} :
-  LocalUpdate (λ x, Lv (frac_car x)) (frac_map L).
-Proof.
-  split; first apply _. intros n [p a] [q b]; simpl.
-  intros ? [??]; constructor; [done|by apply (local_updateN L)].
-Qed.
-
-(** Updates *)
-Lemma frac_update (a1 a2 : A) p : a1 ~~> a2 → Frac p a1 ~~> Frac p a2.
-Proof.
-  intros Ha n mz [??]; split; first by destruct mz.
-  pose proof (Ha n (frac_car <$> mz)); destruct mz; naive_solver.
-Qed.
-End cmra.
-
-Arguments fracR : clear implicits.
-
-(* Functor *)
-Instance frac_map_cmra_monotone {A B : cmraT} (f : A → B) :
-  CMRAMonotone f → CMRAMonotone (frac_map f).
-Proof.
-  split; try apply _.
-  - intros n [p a]; destruct 1; split; simpl in *; auto using validN_preserving.
-  - intros [q1 a1] [q2 a2] [[q3 a3] [??]]; setoid_subst.
-    destruct (included_preserving f a1 (a1 ⋅ a3)) as [b ?].
-    { by apply cmra_included_l. }
-    by exists (Frac q3 b); constructor.
-Qed.
-
-Program Definition fracRF (F : rFunctor) : rFunctor := {|
-  rFunctor_car A B := fracR (rFunctor_car F A B);
-  rFunctor_map A1 A2 B1 B2 fg := fracC_map (rFunctor_map F fg)
-|}.
-Next Obligation.
-  by intros F A1 A2 B1 B2 n f g Hfg; apply fracC_map_ne, rFunctor_ne.
-Qed.
-Next Obligation.
-  intros F A B x. rewrite /= -{2}(frac_map_id x).
-  apply frac_map_ext=>y; apply rFunctor_id.
-Qed.
-Next Obligation.
-  intros F A1 A2 A3 B1 B2 B3 f g f' g' x. rewrite /= -frac_map_compose.
-  apply frac_map_ext=>y; apply rFunctor_compose.
-Qed.
-
-Instance fracRF_contractive F :
-  rFunctorContractive F → rFunctorContractive (fracRF F).
-Proof.
-  by intros ? A1 A2 B1 B2 n f g Hfg; apply fracC_map_ne, rFunctor_contractive.
 Qed.
